part of ber_tlv_tag_serialize proof

src/Lib/DWT/ExecBer_tlv_tag_serialize.v
@@ -1,49 +1,37 @@
-Require Import Core.Core.
+Require Import Core.Core Core.Notations.
 
 Definition byte_length z :=
-  let fix byte_length n i z l:= 
-      match n with
-      | O => l
-      | S n =>
-        if z / 2^i =? 0 
-        then l 
-        else byte_length n (i + 7) z (l + 1)
-      end
-  in byte_length 4%nat 7 z 1.
-
-Definition byte_length_shift z :=
   let fix byte_length n z i l :=
       match n with
       | O => l
-      | S n =>  
-        if Z.shiftr z i =? 0
-        then l else 
-          byte_length n z (i + 7) (l + 1)
+      | S n => if z >> i =? 0
+               then l 
+               else byte_length n z (i + 7) (l + 1)
       end in
   byte_length 4%nat z 7 1.
 
 Definition serialize_tag tval :=
 let fix serialize_tag n i tval :=
   match n with
-  | O => [Z.land tval 127]
-  | S n => (Z.lor 128 (Z.land (Z.shiftr tval i) 127)) :: serialize_tag n (i - 7) tval
+  | O => [tval & 127]
+  | S n => (128 or (tval >> i & 127)) :: serialize_tag n (i - 7) tval
   end in 
- let req_size := byte_length_shift tval in 
+ let req_size := byte_length tval in 
  serialize_tag (Z.to_nat (req_size - 1)) ((req_size * 7) - 7)%Z tval.
     
-Definition ber_tlv_tag_serialize (tag size : Z) : list byte * Z :=
-  let tclass := Z.land tag 3 in 
-  let tval := Z.shiftr tag 2 in
+Definition ber_tlv_tag_serialize (tag size : Z): list byte * Z :=
+  let tclass := tag & 3 in 
+  let tval := tag >> 2 in
   if tval <=? 30 then (* Encoded in 1 octet *)
     if negb (size =? 0) 
-    then ([Byte.repr (Z.lor (Z.shiftl tclass 6) tval)], 1)
+    then ([Byte.repr ((tclass << 6) or tval)], 1)
     else ([], 1)
   else (* Encoded in > 1 octet *) 
     let required_size := byte_length tval in
     if negb (size =? 0) 
-       then let buf0 := (Z.lor (Z.shiftl tclass 6) 31) in
+       then let buf0 := (tclass << 6) or 31 in
             if size - 1 <? required_size 
-            then ([], required_size + 1)
+            then ([Byte.repr buf0], required_size + 1)
             else
             (map Byte.repr (buf0 :: (serialize_tag tag)), required_size + 1)
        else ([], required_size + 1).
