src/Lib/DWT/VSTber_tlv_tag_serialize.v
@@ -1,4 +1,4 @@
-Require Import Core.Core Core.StructNormalizer VstLib DWT.Exec 
+Require Import Core.Core  Core.VstTactics Core.StructNormalizer VstLib DWT.Exec 
         ErrorWithWriter.
 Require Import VST.floyd.proofauto.
 Require Import Clight.ber_tlv_tag ExecBer_tlv_tag_serialize.
@@ -8,14 +8,86 @@ Definition Vprog : varspecs. Proof. mk_varspecs prog. Defined.
 
 Definition ber_tlv_tag_serialize_spec : ident * funspec :=
   DECLARE _ber_tlv_tag_serialize
-  WITH tag: Z, bufp : val, size : Z
+  WITH tag: Z, bufp : val, size : Z, buf_size : Z
   PRE[tuint, tptr tvoid, tuint]
-    PROP()
+    PROP(0 <= size < Int.modulus;
+         32 <= buf_size )
     PARAMS(Vint (Int.repr tag); bufp; Vint (Int.repr size))
     GLOBALS()
-    SEP(data_at_ Tsh tvoid bufp)
-    POST[tuint]
+    SEP(data_at_ Tsh (tarray tuchar buf_size) bufp)
+  POST[tuint]
     let (ls, z) := ber_tlv_tag_serialize tag size in
-      PROP()
-      LOCAL(temp ret_temp (Vint (Int.repr z)))
-      SEP(data_at Tsh (tarray tuint (Zlength ls)) (map Vubyte ls) bufp).
+    PROP()
+    LOCAL(temp ret_temp (Vint (Int.repr z)))
+    SEP(if eq_dec ls [] 
+        then data_at_ Tsh (tarray tuchar buf_size) bufp 
+        else data_at Tsh (tarray tuint (Zlength ls)) (map Vubyte ls) bufp).
+
+Definition Gprog := ltac:(with_library prog [ber_tlv_tag_serialize_spec]).
+
+Theorem ber_tlv_tag_serialize_correct : 
+  semax_body Vprog Gprog (normalize_function f_ber_tlv_tag_serialize composites)
+             ber_tlv_tag_serialize_spec.
+Proof.
+  start_function.
+  repeat forward.
+  forward_if.
+  - forward_if (
+       let (ls, z) := ber_tlv_tag_serialize tag size in
+       PROP()
+       LOCAL()
+       SEP(if eq_dec size 0 
+           then data_at_ Tsh (tarray tuchar buf_size) bufp 
+           else data_at Tsh (tarray tuint (Zlength ls)) (map Vubyte ls) bufp)).
+    + forward. break_let. 
+      rewrite_if_b. entailer!.
+       unfold upd_Znth.
+      break_if.
+      autorewrite with sublist.
+      entailer!.
+      unfold ber_tlv_tag_serialize in *.
+      replace (Z.shiftr tag 2 <=? 30) with true in *.
+      break_if.
+      replace l with [Byte.repr (Z.lor (Z.shiftl (Z.land tag 3) 6) (Z.shiftr tag 2))].
+      entailer!.
+      unfold upd_Znth. 
+      all: admit.
+    + forward. break_let. entailer!. 
+      break_if. entailer.
+      assert (Int.unsigned (Int.repr size) = Int.unsigned (Int.repr 0)).
+      f_equal. auto.
+      repeat rewrite Int.unsigned_repr_eq in *.
+      rewrite Zmod_small in *.
+      rewrite Zmod_small in *.
+      nia.
+      rep_omega.
+      nia.
+    + unfold POSTCONDITION.
+      unfold abbreviate. 
+      break_let.
+      forward.
+      rewrite_if_b.
+      break_if.
+      unfold ber_tlv_tag_serialize in *.
+      replace (Z.shiftr tag 2 <=? 30) with true in *.
+      admit.
+      admit.
+      unfold ber_tlv_tag_serialize in *.
+      replace (Z.shiftr tag 2 <=? 30) with true in *.
+      (* rewrite Heqb in *.
+      inversion Heqp.
+      break_if.
+      congruence.
+      entailer!. *)
+      admit.
+      admit.
+  - forward_if True.
+    + forward.
+      forward.
+            admit.
+    + forward. entailer!.
+    + repeat forward.
+      (* loop *)
+      admit.
+Admitted.
+
