src/Core/VstTactics.v
@@ -1,0 +1,11 @@
+Require Import VST.floyd.proofauto.
+
+Ltac forward_empty_loop :=
+      match goal with
+      | [ _ : _ |- semax _ ?Pre (Ssequence (Sloop Sskip Sbreak) _) _ ] =>
+          forward_loop Pre break: Pre; try forward ; try entailer! 
+      end. 
+
+Ltac rewrite_if_b := 
+  try rewrite if_true in * by (reflexivity || assumption); 
+  try rewrite if_false in * by (reflexivity || assumption).
